bedrock2/src/bedrock2/Memory.v
@@ -10,16 +10,112 @@ Require Import BinIntDef coqutil.Word.Interface coqutil.Word.LittleEndianList.
 Require Import bedrock2.Notations bedrock2.Syntax.
 Require Import coqutil.Byte.
 Require Import coqutil.Map.OfListWord.
+Require Import coqutil.Word.Bitwidth.
 
 Open Scope Z_scope.
 
 Definition bytes_per_word(width: Z): Z := (width + 7) / 8.
 
+Definition bytes_per {width} {BW : Bitwidth.Bitwidth width} sz :=
+  match sz with
+    | access_size.one => 1 | access_size.two => 2 | access_size.four => 4
+    | access_size.word => Z.to_nat (bytes_per_word width)
+  end%nat.
+
+Module Deprecated. Section Memory.
+  Context {width: Z} {BW : Bitwidth.Bitwidth width} {word: word width} {mem: map.map word byte}.
+
+  Definition ftprint(a: word)(n: Z): list word :=
+    List.unfoldn (fun w => word.add w (word.of_Z 1)) (Z.to_nat n) a.
+
+  Definition anybytes(a: word)(n: Z)(m: mem): Prop :=
+    exists bytes: list byte, map.of_disjoint_list_zip (ftprint a n) bytes = Some m.
+
+  Definition footprint(a: word)(sz: nat): tuple word sz :=
+    tuple.unfoldn (fun w => word.add w (word.of_Z 1)) sz a.
+
+  Definition load_bytes(sz: nat)(m: mem)(addr: word): option (tuple byte sz) :=
+    map.getmany_of_tuple m (footprint addr sz).
+
+  Definition unchecked_store_bytes(sz: nat)(m: mem)(a: word)(bs: tuple byte sz): mem :=
+    map.putmany_of_tuple (footprint a sz) bs m.
+
+  Definition store_bytes(sz: nat)(m: mem)(a: word)(v: tuple byte sz): option mem :=
+    match load_bytes sz m a with
+    | Some _ => Some (unchecked_store_bytes sz m a v)
+    | None => None (* some addresses were invalid *)
+    end.
+
+  Definition load_Z(sz: access_size)(m: mem)(a: word): option Z :=
+    match load_bytes (bytes_per sz) m a with
+    | Some bs => Some (LittleEndianList.le_combine (tuple.to_list bs))
+    | None => None
+    end.
+
+  Definition store_Z(sz: access_size)(m: mem)(a: word)(v: Z): option mem :=
+    store_bytes _ m a (tuple.of_list (LittleEndianList.le_split (bytes_per sz) v)).
+
+  Definition load(sz: access_size)(m: mem)(a: word): option word :=
+    match load_Z sz m a with
+    | Some v => Some (word.of_Z v)
+    | None => None
+    end.
+
+  Definition store(sz: access_size)(m: mem)(a: word)(v: word): option mem :=
+    store_Z sz m a (word.unsigned v).
+
+  Lemma load_None: forall sz m a,
+      8 <= width -> (* note: [0 < width] is sufficient *)
+      map.get m a = None ->
+      load sz m a = None.
+  Proof.
+    intros. destruct sz; cbv [load load_Z load_bytes map.getmany_of_tuple footprint bytes_per bytes_per_word tuple.option_all tuple.map tuple.unfoldn];
+    try solve [ rewrite H0; reflexivity].
+    destruct (Z.to_nat ((width + 7) / 8)) eqn: E.
+    - exfalso.
+      assert (0 < (width + 7) / 8) as A. {
+        apply Z.div_str_pos. blia.
+      }
+      change O with (Z.to_nat 0) in E.
+      apply Z2Nat.inj in E; blia.
+    - cbv [tuple.option_all tuple.map tuple.unfoldn].
+      rewrite H0.
+      reflexivity.
+  Qed.
+
+  Context {mem_ok: map.ok mem}.
+  Context {word_ok: word.ok word}.
+
+  Lemma store_preserves_domain: forall sz m a v m',
+      store sz m a v = Some m' -> map.same_domain m m'.
+  Proof.
+    destruct sz;
+      cbv [store store_Z store_bytes bytes_per load_bytes unchecked_store_bytes];
+      intros;
+      (destruct_one_match_hyp; [|discriminate]);
+      inversion_option;
+      subst;
+      eapply map.putmany_of_tuple_preserves_domain;
+      eassumption.
+  Qed.
+
+  Lemma anybytes_unique_domain: forall a n m1 m2,
+      anybytes a n m1 ->
+      anybytes a n m2 ->
+      map.same_domain m1 m2.
+  Proof.
+    unfold anybytes. intros.
+    destruct H as [vs1 ?]. destruct H0 as [vs2 ?].
+    eapply map.of_disjoint_list_zip_same_domain; eassumption.
+  Qed.
+
+End Memory. End Deprecated.
+
 Global Notation "xs $@ a" := (map.of_list_word_at a xs) (at level 10, format "xs $@ a").
 Local Infix "$+" := map.putmany (at level 70).
 
-Module WithoutTuples. Section Memory.
-  Context {width: Z} {word: word width} {mem: map.map word byte}.
+Section Memory.
+  Context {width: Z} {BW : Bitwidth.Bitwidth width} {word: word width} {mem: map.map word byte}.
   Definition footprint (a : word) (n : nat) : list word :=
     List.map (fun i => word.add a (word.of_Z (Z.of_nat i))) (List.seq 0 n).
   Definition load_bytes (m : mem) (a : word) (n : nat) : option (list byte) :=
@@ -31,6 +127,8 @@ Module WithoutTuples. Section Memory.
     | Some _ => Some (unchecked_store_bytes m a bs)
     | None => None (* some addresses were invalid *)
     end.
+  Definition anybytes(a: word)(n: Z)(m: mem): Prop :=
+    exists bs, Z.of_nat (length bs) = n /\ m = bs$@a.
 
   Local Notation "a [ i ]" := (List.nth_error a i) (at level 9, format "a [ i ]").
 
@@ -81,7 +179,7 @@ Module WithoutTuples. Section Memory.
   Proof.
     destruct (load_bytes m a n) eqn:HX; eauto.
     eapply load_bytes_None in HX; destruct HX as (?&?&?). firstorder congruence.
-    exact nil.
+    all : exact nil.
   Qed.
 
   Import Word.Properties.
@@ -108,81 +206,10 @@ Module WithoutTuples. Section Memory.
       cbv [word.wrap]; rewrite Z.mod_small, Znat.Nat2Z.id; eauto; blia. }
     congruence.
   Qed.
-End Memory. End WithoutTuples.
 
-Section Memory.
-  Context {width: Z} {word: word width} {mem: map.map word byte}.
-
-  Definition ftprint(a: word)(n: Z): list word :=
-    List.unfoldn (fun w => word.add w (word.of_Z 1)) (Z.to_nat n) a.
-
-  Definition anybytes(a: word)(n: Z)(m: mem): Prop :=
-    exists bytes: list byte, map.of_disjoint_list_zip (ftprint a n) bytes = Some m.
-
-  Definition footprint(a: word)(sz: nat): tuple word sz :=
-    tuple.unfoldn (fun w => word.add w (word.of_Z 1)) sz a.
-
-  Definition load_bytes(sz: nat)(m: mem)(addr: word): option (tuple byte sz) :=
-    map.getmany_of_tuple m (footprint addr sz).
-
-  Definition unchecked_store_bytes(sz: nat)(m: mem)(a: word)(bs: tuple byte sz): mem :=
-    map.putmany_of_tuple (footprint a sz) bs m.
-
-  Definition store_bytes(sz: nat)(m: mem)(a: word)(v: tuple byte sz): option mem :=
-    match load_bytes sz m a with
-    | Some _ => Some (unchecked_store_bytes sz m a v)
-    | None => None (* some addresses were invalid *)
-    end.
-
-  Definition bytes_per sz :=
-    match sz with
-      | access_size.one => 1 | access_size.two => 2 | access_size.four => 4
-      | access_size.word => Z.to_nat (bytes_per_word width)
-    end%nat.
-
-  Definition load_Z(sz: access_size)(m: mem)(a: word): option Z :=
-    match load_bytes (bytes_per sz) m a with
-    | Some bs => Some (LittleEndianList.le_combine (tuple.to_list bs))
-    | None => None
-    end.
-
-  Definition store_Z(sz: access_size)(m: mem)(a: word)(v: Z): option mem :=
-    store_bytes _ m a (tuple.of_list (LittleEndianList.le_split (bytes_per sz) v)).
-
-  Definition load(sz: access_size)(m: mem)(a: word): option word :=
-    match load_Z sz m a with
-    | Some v => Some (word.of_Z v)
-    | None => None
-    end.
-
-  Definition store(sz: access_size)(m: mem)(a: word)(v: word): option mem :=
-    store_Z sz m a (word.unsigned v).
-
-  Lemma load_None: forall sz m a,
-      8 <= width -> (* note: [0 < width] is sufficient *)
-      map.get m a = None ->
-      load sz m a = None.
+  Lemma footprint_deprecated a s : tuple.to_list (Deprecated.footprint a s) = footprint a s.
   Proof.
-    intros. destruct sz; cbv [load load_Z load_bytes map.getmany_of_tuple footprint bytes_per bytes_per_word tuple.option_all tuple.map tuple.unfoldn];
-    try solve [ rewrite H0; reflexivity].
-    destruct (Z.to_nat ((width + 7) / 8)) eqn: E.
-    - exfalso.
-      assert (0 < (width + 7) / 8) as A. {
-        apply Z.div_str_pos. blia.
-      }
-      change O with (Z.to_nat 0) in E.
-      apply Z2Nat.inj in E; blia.
-    - cbv [tuple.option_all tuple.map tuple.unfoldn].
-      rewrite H0.
-      reflexivity.
-  Qed.
-
-  Context {mem_ok: map.ok mem}.
-  Context {word_ok: word.ok word}.
-
-  Lemma footprint_WithoutTuples a s : tuple.to_list (footprint a s) = WithoutTuples.footprint a s.
-  Proof.
-    cbv [footprint WithoutTuples.footprint].
+    cbv [Deprecated.footprint footprint].
     revert a; induction s; cbn; trivial; 
     intros; f_equal.
     2: rewrite <-List.seq_shift, List.map_map, IHs; eapply List.map_ext; intros i.
@@ -193,11 +220,11 @@ Section Memory.
     f_equal. blia.
   Qed.
 
-  Lemma load_bytes_WithoutTuples s m a :
-    option_map tuple.to_list (load_bytes s m a) = WithoutTuples.load_bytes m a s.
+  Lemma load_bytes_deprecated s m a :
+    option_map tuple.to_list (Deprecated.load_bytes s m a) = load_bytes m a s.
   Proof.
-    cbv [load_bytes WithoutTuples.load_bytes map.getmany_of_tuple ].
-    rewrite <- footprint_WithoutTuples; generalize (footprint a s); clear a.
+    cbv [Deprecated.load_bytes load_bytes map.getmany_of_tuple ].
+    rewrite <- footprint_deprecated; generalize (Deprecated.footprint a s); clear a.
     induction s; cbn; trivial; intros (p&t').
     destruct map.get; cbn; trivial.
     rewrite <-IHs.
@@ -208,11 +235,11 @@ Section Memory.
     if Nat.eqb i O then Some x else List.nth_error xs (pred i).
   Proof. destruct i; trivial. Qed.
 
-  Lemma unchecked_store_bytes_WithoutTuples s m a v :
-    unchecked_store_bytes s m a v
-    = WithoutTuples.unchecked_store_bytes m a (tuple.to_list v).
+  Lemma unchecked_store_bytes_deprecated s m a v :
+    Deprecated.unchecked_store_bytes s m a v
+    = unchecked_store_bytes m a (tuple.to_list v).
   Proof.
-    cbv [unchecked_store_bytes WithoutTuples.unchecked_store_bytes footprint].
+    cbv [Deprecated.unchecked_store_bytes unchecked_store_bytes Deprecated.footprint].
     revert a; revert v; revert m. induction s; cbn; intros.
     { erewrite map.of_list_word_nil, map.putmany_empty_r; trivial. }
     destruct v as [v vs].
@@ -237,36 +264,13 @@ Section Memory.
     rewrite !Zminus_mod_idemp_l, !Zminus_mod_idemp_r, Z.sub_add_distr; trivial.
   Qed.
 
-  Lemma store_bytes_WithoutTuples s m a v :
-    store_bytes s m a v = WithoutTuples.store_bytes m a (tuple.to_list v).
+  Lemma store_bytes_deprecated s m a v :
+    Deprecated.store_bytes s m a v = store_bytes m a (tuple.to_list v).
   Proof.
-    cbv [store_bytes WithoutTuples.store_bytes].
-    rewrite tuple.length_to_list, <-load_bytes_WithoutTuples; cbv [option_map].
-    destruct load_bytes in *; f_equal.
-    eapply unchecked_store_bytes_WithoutTuples.
-  Qed.
-
-  Lemma store_preserves_domain: forall sz m a v m',
-      store sz m a v = Some m' -> map.same_domain m m'.
-  Proof.
-    destruct sz;
-      cbv [store store_Z store_bytes bytes_per load_bytes unchecked_store_bytes];
-      intros;
-      (destruct_one_match_hyp; [|discriminate]);
-      inversion_option;
-      subst;
-      eapply map.putmany_of_tuple_preserves_domain;
-      eassumption.
-  Qed.
-
-  Lemma anybytes_unique_domain: forall a n m1 m2,
-      anybytes a n m1 ->
-      anybytes a n m2 ->
-      map.same_domain m1 m2.
-  Proof.
-    unfold anybytes. intros.
-    destruct H as [vs1 ?]. destruct H0 as [vs2 ?].
-    eapply map.of_disjoint_list_zip_same_domain; eassumption.
+    cbv [Deprecated.store_bytes store_bytes].
+    rewrite tuple.length_to_list, <-load_bytes_deprecated; cbv [option_map].
+    destruct Deprecated.load_bytes in *; f_equal.
+    eapply unchecked_store_bytes_deprecated.
   Qed.
 
 End Memory.
