bedrock2/src/bedrock2/Map/SeparationLogic.v
@@ -44,7 +44,7 @@ Section SepProperties.
   Proof. cbv [iff1 sep split]; t; eauto 15 using eq_sym, putmany_assoc, ((fun m1 m2 m3 => proj2 (disjoint_putmany_l m1 m2 m3))), ((fun m1 m2 m3 => proj2 (disjoint_putmany_r m1 m2 m3))). Qed.
 
   Lemma get_ptsto k v m (H : ptsto k v m) : get m k = Some v.
-  Proof. rewrite H, get_put_same; trivial. Qed.
+  Proof. rewrite <-H, get_put_same; trivial. Qed.
   Lemma get_sep k v R m (H : sep (ptsto k v) R m) : get m k = Some v.
   Proof.
     destruct H as (mk&mR&H&Hp&HR); eapply get_ptsto in Hp; subst.
@@ -70,7 +70,7 @@ Section SepProperties.
   Lemma sep_put k v m v_old R (H : sep (ptsto k v_old) R m) : sep (ptsto k v) R (put m k v).
   Proof.
     eapply sep_comm in H; eapply sep_comm.
-    destruct H as (mR&mk&[Heq Hd]&HR&Hp); cbv [ptsto] in Hp; subst mk; subst m.
+    destruct H as (mR&mk&[Heq Hd]&HR&Hp); cbv [ptsto exactly] in Hp; subst mk; subst m.
     exists mR, (put empty k v); split; [|solve[repeat split; trivial]]; split.
     { eapply map_ext; intro k'; destruct (key_eq_dec k' k); try subst k';
         rewrite ?get_put_same, ?get_put_diff by trivial.
