bedrock2/src/bedrock2/ptsto_bytes.v
@@ -1,28 +1,18 @@
-Require Import coqutil.Map.Interface coqutil.Map.Properties bedrock2.Map.Separation bedrock2.Map.SeparationLogic bedrock2.Lift1Prop bedrock2.Array.
-Require Import bedrock2.Memory.
-Require Import Coq.Lists.List Coq.ZArith.ZArith.
-Require Import coqutil.Word.Interface coqutil.Word.Properties coqutil.Map.Interface.
-Require Import coqutil.Z.div_mod_to_equations.
-Import HList List PrimitivePair.
-Require Import coqutil.Z.Lia.
-Require Import coqutil.Byte.
-Require Import Coq.ZArith.ZArith.
+Require Import Coq.ZArith.BinInt Coq.setoid_ring.Ring_tac.
+Require Import coqutil.Word.Interface coqutil.Word.Properties Coq.Init.Byte.
+Require Import coqutil.Map.Interface bedrock2.Map.SeparationLogic. 
 Import Map.Separation.Coercions.
-
-Open Scope Z_scope.
+Require Import bedrock2.Memory.
+Local Open Scope Z_scope.
 
 Require Import coqutil.Map.OfListWord.
-Require Import Ring_tac.
 Section WithWord.
   Local Coercion Z.of_nat : nat >-> Z.
-  Local Infix "$+" := map.putmany (at level 70).
-  Local Notation "xs $@ a" := (map.of_list_word_at a xs) (at level 10, format "xs $@ a").
-  Local Infix "*" := sep : type_scope.
   Local Open Scope sep_scope.
   Context {width : Z} {word : Word.Interface.word width} {word_ok : word.ok word}.
   Context [value] [map : map.map word value] {ok : map.ok map}.
   Add Ring __wring: (@word.ring_theory width word word_ok).
-  Lemma sep_eq_of_list_word_at_app (a : word) (xs ys : list value)
+  Lemma sep_of_app (a : word) (xs ys : list value)
     lxs (Hlxs : Z.of_nat (length xs) = lxs) (Htotal : length xs + length ys <= 2^width)
     : Lift1Prop.iff1 ((xs ++ ys)$@a)
       (sep (xs$@a) (ys$@(word.add a (word.of_Z lxs)))).
@@ -34,234 +24,33 @@ Section WithWord.
     erewrite map.of_list_word_at_app_n by eauto; reflexivity.
   Qed.
 
-  Lemma list_word_at_app_of_adjacent_eq (a b : word) (xs ys : list value)
+  Lemma app_of_sep (a b : word) (xs ys : list value)
     (Hl: word.unsigned (word.sub b a) = Z.of_nat (length xs))
     (Htotal : length xs + length ys <= 2^width)
     : Lift1Prop.iff1 (xs$@a * ys$@b) ((xs++ys)$@a).
   Proof.
     etransitivity.
-    2:symmetry; eapply sep_eq_of_list_word_at_app; trivial.
+    2:symmetry; eapply sep_of_app; trivial.
     do 3 Morphisms.f_equiv. rewrite <-Hl, word.of_Z_unsigned. ring.
-  Qed.
-
-  Lemma array1_iff_eq_of_list_word_at (a : word) (bs : list value)
-    (H : length bs <= 2 ^ width) :
-    iff1 (array ptsto (word.of_Z 1) a bs) (bs$@a).
-  Proof.
-    symmetry.
-    revert H; revert a; induction bs; cbn [array]; intros.
-    { rewrite map.of_list_word_nil; cbv [emp iff1 sepclause_of_map]; intuition auto. }
-    { etransitivity.
-      2: eapply Proper_sep_iff1.
-      3: eapply IHbs.
-      2: reflexivity.
-      2: cbn [length] in H; blia.
-      change (a::bs) with (cons a nil++bs).
-      rewrite map.of_list_word_at_app.
-      etransitivity.
-      1: eapply sep_eq_putmany, map.adjacent_arrays_disjoint; cbn [length] in *; blia.
-      etransitivity.
-      2:eapply sep_comm.
-      Morphisms.f_equiv.
-      rewrite map.of_list_word_singleton; try exact _.
-      cbv [ptsto iff1]; intuition auto. }
   Qed.
 End WithWord.
 
-Section Scalars.
+Section WithMem.
   Context {width : Z} {word : Word.Interface.word width} {word_ok : word.ok word}.
-
   Context {mem : map.map word byte} {mem_ok : map.ok mem}.
-
-  Definition ptsto_bytes_deprecated (n : nat) (addr : word) (value : tuple byte n) : mem -> Prop :=
-    array ptsto (word.of_Z 1) addr (tuple.to_list value).
-  Local Notation ptsto_bytes := ptsto_bytes_deprecated.
-
-  Lemma ptsto_bytes_iff_eq_of_list_word_at (n : nat) (addr : word) (value : tuple byte n)
-    (H : (Z.of_nat n <= 2 ^ width)%Z) :
-    iff1 (ptsto_bytes_deprecated n addr value) (tuple.to_list value$@addr).
-  Proof. eapply array1_iff_eq_of_list_word_at; rewrite ?tuple.length_to_list; trivial. Qed.
-
-  Lemma WithoutTuples__load_bytes_of_sep a n bs (Hn : length bs = n) (Hl : Z.of_nat n <= 2^width)
-    R (m : mem) (Hsep : sep (bs$@a) R m) : Memory.WithoutTuples.load_bytes m a n = Some bs.
+  Lemma load_bytes_of_sep a n bs (Hn : length bs = n) (Hl : Z.of_nat n <= 2^width)
+    R (m : mem) (Hsep : sep (bs$@a) R m) : Memory.load_bytes m a n = Some bs.
   Proof.
     eapply sep_comm in Hsep.
     case Hsep as (mR&?&(?&?)&?&Hmbs); destruct Hmbs; subst m.
-    eauto using WithoutTuples.load_bytes_of_putmany_bytes_at.
+    eauto using load_bytes_of_putmany_bytes_at.
   Qed.
 
-  Lemma load_bytes_of_sep a n bs R m
-    (Hsep : sep (ptsto_bytes n a bs) R m)
-    : Memory.load_bytes n m a = Some bs.
-  Proof.
-    cbv [load_bytes footprint].
-    revert bs m R a Hsep.
-    induction n; [solve[cbn; intros []; trivial]|].
-    intros [b0 bs] m R a Hsep.
-    cbn in Hsep; eapply SeparationLogic.sep_assoc in Hsep.
-    cbn [map.getmany_of_tuple tuple.option_all tuple.map tuple.unfoldn].
-    erewrite SeparationLogic.get_sep by exact Hsep.
-    match goal with IH: _ |- _ => setoid_rewrite IH; [exact eq_refl|] end.
-    unfold ptsto_bytes.
-    SeparationLogic.ecancel_assumption.
-  Qed.
-
-  Local Arguments Z.of_nat: simpl never.
-
-  Lemma invert_getmany_of_tuple_Some_footprint
-    (n : nat) (a: word) (vs : tuple byte (S n)) (m : mem)
-    (D: Z.of_nat n < 2 ^ width)
-    (H: map.getmany_of_tuple m (footprint a (S n)) = Some vs):
-    exists m', map.split m (map.put map.empty a (pair._1 vs)) m' /\
-      map.getmany_of_tuple m' (footprint (word.add a (word.of_Z 1)) n) = Some (pair._2 vs).
-  Proof.
-    apply map.invert_getmany_of_tuple_Some in H. destruct H as [B1 B2].
-    exists (map.remove m a).
-    repeat split.
-    - apply map.map_ext. intros k.
-      pose proof (map.putmany_spec (map.put map.empty a (pair._1 vs)) (map.remove m a) k) as P.
-      destruct P as [[v [A B]] | [A B]].
-      + rewrite B.
-        destruct (word.eqb a k) eqn: E.
-        * apply word.eqb_true in E. subst k.
-          rewrite map.get_remove_same in A. discriminate.
-        * apply word.eqb_false in E.
-          rewrite map.get_remove_diff in A by congruence. exact A.
-      + rewrite B.
-        destruct (word.eqb a k) eqn: E.
-        * apply word.eqb_true in E. subst k.
-          rewrite map.get_put_same. exact B1.
-        * apply word.eqb_false in E.
-          rewrite map.get_remove_diff in A by congruence.
-          rewrite map.get_put_diff by congruence.
-          rewrite map.get_empty. exact A.
-    - unfold map.disjoint. intros k ? ? G1 G2.
-      destruct (word.eqb a k) eqn: E.
-        * apply word.eqb_true in E. subst k.
-          rewrite map.get_remove_same in G2. discriminate.
-        * apply word.eqb_false in E.
-          rewrite map.get_put_diff in G1 by congruence.
-          rewrite map.get_empty in G1. discriminate.
-    - simpl in B2.
-      clear -B2 mem_ok word_ok D. destruct vs as [v vs]. simpl in *.
-      assert (0 < 1) as Y by blia.
-      assert (1 + Z.of_nat n <= 2 ^ width)%Z as X by blia. clear D.
-      revert Y X B2. generalize 1%Z as d. clear v. revert a vs. induction n;
-      intros a vs d Y X B2; simpl in *.
-      + destruct vs. reflexivity.
-      + apply map.invert_getmany_of_tuple_Some in B2. simpl in B2. destruct B2 as [A B].
-        destruct vs as [v vs]. simpl in *.
-        apply map.build_getmany_of_tuple_Some; simpl.
-        * rewrite map.get_remove_diff; [assumption|].
-          clear -X Y word_ok.
-          intro C.
-          apply (f_equal word.unsigned) in C.
-          rewrite word.unsigned_add in C.
-          rewrite <- word.wrap_unsigned in C at 2.
-          apply Z.sub_move_0_r in C.
-          apply (f_equal (fun x => x mod (2 ^ width))) in C.
-          change (0 mod 2 ^ width) with 0 in C.
-          unfold word.wrap in C.
-          rewrite <- Zminus_mod in C.
-          rewrite Z.add_simpl_l in C.
-          rewrite word.unsigned_of_Z in C.
-          unfold word.wrap in C.
-          rewrite Z.mod_mod in C by blia.
-          apply Z.mod_divide in C; [|blia].
-          unfold Z.divide in C.
-          destruct C as [k C].
-          subst d.
-          assert (0 < 2 ^ width). {
-            pose proof word.width_pos.
-            apply Z.pow_pos_nonneg; blia.
-          }
-          assert (0 < k) by Lia.nia.
-          Lia.nia.
-        * match goal with IH: _ |- _ => specialize (IH a vs (d + 1)%Z); rename IH into IHn end.
-          replace (word.add a (word.of_Z (d + 1)))
-            with (word.add (word.add a (word.of_Z d)) (word.of_Z 1)) in IHn.
-          { apply IHn; blia || assumption. }
-          { rewrite (morph_add word.ring_morph). rewrite word.add_assoc. reflexivity. }
-  Qed.
-
-  Lemma sep_of_load_bytes_aux: forall (n: nat) (a: word) (bs: tuple byte n) (m: mem) (Q: mem -> Prop),
-      Z.of_nat n <= 2 ^ width ->
-      sep (fun m0 => Memory.load_bytes n m0 a = Some bs) Q m ->
-      exists R, sep (ptsto_bytes n a bs) (sep R Q) m.
-  Proof.
-    cbv [load_bytes footprint]. unfold ptsto_bytes.
-    intro n; induction n; intros.
-    - cbv [ptsto_bytes array tuple.to_list].
-      simpl in *. unfold map.getmany_of_tuple, tuple.option_all in *.
-      match goal with
-      | H: sep _ _ _ |- _ => destruct H as (mp & mq & A & B & C)
-      end.
-      exists (eq mp).
-      apply sep_emp_l. split; auto.
-      unfold sep. eauto.
-    - match goal with
-      | H: sep _ _ _ |- _ => destruct H as (mp & mq & A & B & C)
-      end.
-      apply invert_getmany_of_tuple_Some_footprint in B; [|blia].
-      destruct B as (mo & B1 & B2).
-      match goal with
-      | x: tuple _ (S _) |- _ => destruct x as [b bs]; simpl in *
-      end.
-
-      Fail (* TODO ecancel_assumption why does it fail? *)
-      edestruct IHn as [R IH]; [..|exists R; ecancel_assumption].
-
-      Ltac ecancel_assumption_fix_just_for_here :=
-        seplog;
-        simple refine (cancel_seps_at_indices 0 1 _ _ _ _);
-        cbn [SeparationLogic.firstn SeparationLogic.skipn SeparationLogic.app SeparationLogic.hd SeparationLogic.tl];
-        [exact (RelationClasses.reflexivity _)|];
-        ecancel.
-
-      edestruct IHn as [R IH]; [..|exists R; ecancel_assumption_fix_just_for_here].
-      + blia.
-      + match goal with
-        | |- sep ?BS (sep ?P ?Q) ?m => assert (sep (sep P BS) Q m); [|ecancel_assumption]
-        end.
-        unfold sep, ptsto, footprint in *. eauto 10.
-  Qed.
-
-  (* The side condition is actually needed: If n was bigger than 2^width,
-     ptsto_bytes would star together the same address more than once. *)
-  Lemma sep_of_load_bytes: forall (n: nat) (a: word) (bs: tuple byte n) (m: mem),
-      Z.of_nat n <= 2 ^ width ->
-      Memory.load_bytes n m a = Some bs ->
-      exists R, sep (ptsto_bytes n a bs) R m.
-  Proof.
-    intros. edestruct sep_of_load_bytes_aux as [R P].
-    - eassumption.
-    - apply sep_comm. apply sep_emp_l. split; [apply I|eassumption].
-    - eexists; ecancel_assumption.
-  Qed.
-
-  Lemma unchecked_store_bytes_of_sep(a: word)(n: nat)(oldbs bs: tuple byte n)(R: mem -> Prop)(m: mem)
-    (Hsep : sep (ptsto_bytes n a oldbs) R m)
-    : sep (ptsto_bytes n a bs) R (Memory.unchecked_store_bytes n m a bs).
-  Proof.
-    revert oldbs bs m R a Hsep; induction n; [solve[cbn; intros []; trivial]|].
-    intros [oldb0 oldbs] [b0 bs] m R a Hsep.
-    cbn in *.
-    apply sep_assoc.
-    eapply sep_put.
-    apply sep_assoc in Hsep.
-    match goal with
-    | IH: _ |- _ => unshelve epose proof (IH oldbs bs m _ (word.add a (word.of_Z 1)) _)
-    end.
-    - shelve.
-    - unfold ptsto_bytes. ecancel_assumption.
-    - seplog.
-  Qed.
-
-  Lemma WithoutTuples__unchecked_store_bytes_of_sep(a: word)(oldbs bs: list byte)(R: mem -> Prop)(m: mem)
+  Lemma unchecked_store_bytes_of_sep(a: word)(oldbs bs: list byte)(R: mem -> Prop)(m: mem)
     (Hsep : sep (oldbs$@a) R m)(H:length bs = length oldbs)
-    : sep (bs$@a) R (Memory.WithoutTuples.unchecked_store_bytes m a bs).
+    : sep (bs$@a) R (Memory.unchecked_store_bytes m a bs).
   Proof.
-    cbv [WithoutTuples.unchecked_store_bytes].
+    cbv [unchecked_store_bytes].
     case Hsep as (mo&mR&(?&?)&?&?); subst m.
     destruct H2. (* subst mo *)
     eexists (bs$@a), mR; Tactics.ssplit; trivial; try reflexivity.
@@ -270,37 +59,18 @@ Section Scalars.
       intros k v1 v2; specialize (H1 k).
       erewrite map.get_of_list_word_at in *.
       intros HSome.
-      eapply nth_error_Some_bound_index in HSome.
-      destruct nth_error eqn:Hd in H1; eauto.
-      eapply nth_error_None in Hd; blia. }
+      eapply List.nth_error_Some_bound_index in HSome.
+      destruct List.nth_error eqn:Hd in H1; eauto.
+      eapply List.nth_error_None in Hd; Lia.lia. }
     split; trivial.
     rewrite <-Properties.map.putmany_assoc.
-    rewrite (Properties.map.putmany_comm mR) by (eapply map.disjoint_comm; assumption).
+    rewrite (Properties.map.putmany_comm mR) by (eapply Properties.map.disjoint_comm; assumption).
     rewrite Properties.map.putmany_assoc.
     f_equal.
     eapply map.map_ext; intros k.
     erewrite Properties.map.get_putmany_dec; case map.get eqn:?; trivial.
     erewrite map.get_of_list_word_at in *.
-    erewrite nth_error_None in *.
-    blia.
+    erewrite List.nth_error_None in *.
+    Lia.lia.
   Qed.
-
-  Lemma unchecked_store_bytes_of_sep'
-      (a: word)(n: nat)(bs1 bs2: tuple byte n)(R1 R2 F: mem -> Prop)(m: mem):
-      R1 m ->
-      iff1 R1 (sep (ptsto_bytes n a bs1) F) ->
-      iff1 R2 (sep (ptsto_bytes n a bs2) F) ->
-      R2 (Memory.unchecked_store_bytes n m a bs2).
-  Proof. intros A B C. eapply C, unchecked_store_bytes_of_sep, B, A. Qed.
-
-  Lemma store_bytes_of_sep(a: word)(n: nat)(oldbs bs: tuple byte n)(R post: mem -> Prop)(m: mem)
-    (Hsep : sep (ptsto_bytes n a oldbs) R m)
-    (Hpost : forall m, sep (ptsto_bytes n a bs) R m -> post m)
-    : exists m1, Memory.store_bytes n m a bs = Some m1 /\ post m1.
-  Proof.
-    cbv [store_bytes]. erewrite load_bytes_of_sep; eauto using unchecked_store_bytes_of_sep.
-  Qed.
-End Scalars.
-
-#[deprecated(note="Use bs$@a instead; Import bedrock2.Memory bedrock2.Map.Separation.Coercions; use array1_iff_eq_of_list_word_at and ptsto_bytes_iff_eq_of_list_word_at.")]
-Global Notation ptsto_bytes := ptsto_bytes_deprecated.
+End WithMem.
